Traces.v
@@ -1,0 +1,220 @@
+Require Import common.Events.
+Require Import common.Values.
+Require Import common.Globalenvs.
+Require Import cfrontend.Clight.
+Require Import lib.Integers.
+
+Require Import Rustre.Common.
+Require Import Rustre.Ident.
+Require Import Rustre.ObcToClight.Interface.
+
+Require Import List.
+Import List.ListNotations.
+Require Import Instantiator.
+Import Obc.Typ.
+Import Obc.Syn.
+(* Import Obc.Sem. *)
+Import DF.Str.
+Import DF.Syn.
+Import OpAux.
+Import Trans.
+
+Section finite_traces.
+  
+  Variable p: Clight.program.
+  
+  Definition eventval_of_val (v: val): eventval :=
+    match v with 
+    | Vint i => EVint i
+    | Vlong i => EVlong i
+    | Vfloat f => EVfloat f
+    | Vsingle f => EVsingle f
+    | Vptr _ _ => (* Not supported *) EVint Int.zero
+    | Vundef => (* Not supported *) EVint Int.zero
+    end.
+
+  Lemma eventval_of_val_match:
+    forall v t, wt_val v t -> 
+           eventval_match (globalenv p) 
+                          (eventval_of_val v) 
+                          (AST.type_of_chunk (type_chunk t)) v.
+  Proof.
+    destruct v; intros ** Wt; inv Wt; simpl; try econstructor.
+    destruct sz; try destruct sg; econstructor.
+  Qed.
+  
+  Definition load_event_of_val (v: val)(xt: ident * type): event
+    := Event_vload (type_chunk (snd xt))
+                   (glob_id (fst xt)) 
+                   Int.zero (eventval_of_val v).
+
+  Definition store_event_of_val (v: val)(xt: ident * type): event
+    := Event_vstore (type_chunk (snd xt))
+                    (glob_id (fst xt)) 
+                    Int.zero (eventval_of_val v).
+
+  Definition mk_event (f: val -> ident * type -> event)
+             (vs: list val)(args: list (ident * type))
+    := map (fun vxt => f (fst vxt) (snd vxt)) (combine vs args). 
+
+  Definition load_events := mk_event load_event_of_val.
+  Definition store_events := mk_event store_event_of_val.
+
+  Lemma mk_event_nil: forall f vs, mk_event f vs [] = [].
+  Proof. intros; destruct vs; simpl; auto. Qed.
+
+  Lemma mk_event_cons: 
+    forall f v vs xt xts, 
+      mk_event f (v :: vs) (xt :: xts) = f v xt :: mk_event f vs xts.
+  Proof. auto. Qed.
+
+  Corollary load_events_nil : forall vs, load_events vs [] = [].
+  Proof. apply mk_event_nil. Qed.
+
+  Corollary load_events_cons : forall v vs xt xts, 
+      load_events (v :: vs) (xt :: xts) = [load_event_of_val v xt] ++ load_events vs xts.
+  Proof. apply mk_event_cons. Qed.
+
+  Corollary store_events_nil : forall vs, store_events vs [] = [].
+  Proof. apply mk_event_nil. Qed.
+
+  Corollary store_events_cons : forall v vs xt xts, 
+      store_events (v :: vs) (xt :: xts) = [store_event_of_val v xt] ++ store_events vs xts.
+  Proof. apply mk_event_cons. Qed.
+
+End finite_traces.
+
+Section infinite_traces.
+
+  Variable ins : stream (list const).
+  Variable outs : stream (list const).
+
+  Variable xs : list (ident * type).
+  Variable ys : list (ident * type).
+
+  Hypothesis xs_spec: xs <> [].
+  Hypothesis ys_spec: ys <> [].
+
+  Hypothesis Hwt_ins: forall n, wt_vals (map sem_const (ins n)) xs.
+  Hypothesis Hwt_outs: forall n, wt_vals (map sem_const (outs n)) ys.
+
+  Lemma load_events_not_E0: forall n, 
+      load_events (map sem_const (ins n)) xs <> E0.
+  Proof.
+    clear - Hwt_ins xs_spec.
+    intros n; specialize Hwt_ins with n.
+    destruct xs; auto.
+    inv Hwt_ins; rewrite load_events_cons; discriminate.
+  Qed.
+
+  Lemma store_events_not_E0: forall n, 
+      store_events (map sem_const (outs n)) ys <> E0.
+  Proof.
+    clear - Hwt_outs ys_spec.
+    intros n; specialize Hwt_outs with n.
+    destruct ys; auto.
+    inv Hwt_outs; simpl; rewrite store_events_cons; discriminate.
+  Qed.
+
+  CoFixpoint mk_trace (n: nat): traceinf'.
+  clear - mk_trace n ins outs xs ys. 
+  refine(
+      (Econsinf' (load_events (map sem_const (ins n)) xs)
+                 (Econsinf' (store_events (map sem_const (outs n)) ys)
+                            (mk_trace (S n)) _) _));
+    [ apply store_events_not_E0
+    | apply load_events_not_E0 ].
+  Defined.
+
+  Lemma unfold_mk_trace: forall n,
+      traceinf_of_traceinf' (mk_trace n) = 
+      (load_events (map sem_const (ins n)) xs
+                   ++ E0
+                   ++ store_events (map sem_const (outs n)) ys)
+        *** E0
+        *** traceinf_of_traceinf' (mk_trace (S n)).
+  Proof.
+    intro.
+    rewrite E0_left, E0_left_inf, (unroll_traceinf' (mk_trace n)).
+    unfold mk_trace at 1.
+    now rewrite 2!traceinf_traceinf'_app, Eappinf_assoc.
+  Qed.
+
+End infinite_traces.
+
+Section Dataflow.
+  Variable (main: node) (ins outs: stream (list const)).
+  
+  Hypothesis Hwt_ins: forall n, wt_vals (map sem_const (ins n)) main.(n_in).
+  Hypothesis Hwt_outs: forall n, wt_vals (map sem_const (outs n)) main.(n_out).
+
+  Lemma n_in_spec: main.(n_in) <> [].
+  Proof.
+    pose proof (n_ingt0 main) as H.
+    intro E; rewrite E in H; simpl in H.
+    eapply Lt.lt_irrefl; eauto.
+  Qed.
+  
+  Lemma n_out_spec: main.(n_out) <> [].
+  Proof.
+    pose proof (n_outgt0 main) as H.
+    intro E; rewrite E in H; simpl in H.
+    eapply Lt.lt_irrefl; eauto.
+  Qed.
+  
+  Definition trace_node (n: nat): traceinf' :=
+    mk_trace ins outs main.(n_in) main.(n_out) n_in_spec n_out_spec Hwt_ins Hwt_outs n.
+
+End Dataflow.
+
+Section Obc.
+  Variable (m_step: method) (ins outs: stream (list const)).
+
+  Hypothesis in_spec: m_step.(m_in) <> [].
+  Hypothesis out_spec: m_step.(m_out) <> [].
+
+  Hypothesis Hwt_ins: forall n, wt_vals (map sem_const (ins n)) m_step.(m_in).
+  Hypothesis Hwt_outs: forall n, wt_vals (map sem_const (outs n)) m_step.(m_out).
+
+  Definition trace_step (n: nat): traceinf' :=
+    mk_trace ins outs m_step.(m_in) m_step.(m_out) in_spec out_spec Hwt_ins Hwt_outs n.
+
+End Obc.
+
+Section Corres.
+  Variable (main: node) (m_step: method) (ins outs: stream (list const)).
+
+  Hypothesis Hwt_ins: forall n, wt_vals (map sem_const (ins n)) main.(n_in).
+  Hypothesis Hwt_outs: forall n, wt_vals (map sem_const (outs n)) main.(n_out).
+
+  Hypothesis Eq_in: main.(n_in) = m_step.(m_in).
+  Hypothesis Eq_out: main.(n_out) = m_step.(m_out).
+
+  Lemma in_spec: m_step.(m_in) <> [].
+  Proof.
+    rewrite <-Eq_in.
+    pose proof (n_ingt0 main) as H.
+    intro E; rewrite E in H; simpl in H.
+    eapply Lt.lt_irrefl; eauto.
+  Qed.
+  
+  Lemma out_spec: m_step.(m_out) <> [].
+  Proof.
+    rewrite <-Eq_out.
+    pose proof (n_outgt0 main) as H.
+    intro E; rewrite E in H; simpl in H.
+    eapply Lt.lt_irrefl; eauto.
+  Qed.
+
+  Lemma Hwt_ins': forall n, wt_vals (map sem_const (ins n)) m_step.(m_in).
+  Proof. now rewrite <-Eq_in. Qed.
+  
+  Lemma Hwt_outs': forall n, wt_vals (map sem_const (outs n)) m_step.(m_out).
+  Proof. now rewrite <-Eq_out. Qed.
+
+  Lemma trace_equiv:
+    forall n,
+      traceinf_sim' (traceinf_of_traceinf' (trace_node main ins outs Hwt_ins Hwt_outs n)) 
+                    (traceinf_of_traceinf' (trace_step m_step ins outs in_spec out_spec Hwt_ins' Hwt_outs' n)).
+  Admitted.
+End Corres.  
